Lean/Geo.lean
@@ -1,4 +1,5 @@
 -- This module serves as the root of the `Geo` library.
 -- Import modules here that should be built as part of the library.
 import Geo.Naive.TheMainTheorem
+import Geo.Gon.TheMainTheorem
 import Geo.Hexagon.TheMainTheorem
