Lean/Geo/Gon/Assn.lean
@@ -1,0 +1,65 @@
+import Geo.Definitions.CanonicalPoints
+import Geo.Definitions.PtInTriangle
+import Geo.Definitions.Structures
+import Geo.Definitions.OrientationProperties
+import Geo.Definitions.Orientations
+import Geo.Gon.Encoding
+import Geo.KGon.Assn
+import Geo.KGon.Arc
+
+namespace Geo.CanonicalPoints
+open List Classical Point
+attribute [-simp] getElem_fin
+
+theorem isArc.exists_arc {w : CanonicalPoints} {a b c : Fin w.rlen}
+    (ab : a < b) (bc : b < c) (H : isArc w o sz a b c) :
+    ∃ l, l.length = sz ∧ Arc w o (a.succ :: l ++ [b.succ, c.succ]) := by
+  match sz, H with
+  | 0, H => exact ⟨[], rfl, .cons ab.succ₂ H (.one bc.succ₂)⟩
+  | l+1, ⟨bc, d, ad, db, h1, h2⟩ =>
+    let ⟨l, eq, h1'⟩ := h1.exists_arc ad db
+    exact ⟨_, by simp [eq], .concat h1' bc h2⟩
+
+theorem satisfies_arc2 {w : CanonicalPoints} {a b : Fin w.rlen}
+    (ab : a < b) (H : (arc2 o sz a b).eval (w.toPropAssn false)) :
+    ∃ l, l.length = sz ∧ Arc w o (a.succ :: l ++ [b.succ]) := by
+  unfold arc2 at H; split at H
+  · exact ⟨[], rfl, .one ab.succ₂⟩
+  · simp at H; let ⟨c, ⟨ac, cb⟩, H'⟩ := H
+    have ac : a < c := Nat.lt_of_le_of_lt (Nat.le_add_right ..) ac
+    have ⟨l, eq, hl⟩ := ((eval_arc _ ac cb).1 H').exists_arc ac cb
+    exact ⟨l ++ [c.succ], by simp [eq], by simpa using hl⟩
+
+theorem satisfies_noKGon2Arc {w : CanonicalPoints}
+    (H : ∀ a b : Fin w.rlen, ∀ l1 l2, l1.length = sz1 → l2.length = sz2 →
+      Arc w .ccw (a.succ :: l1 ++ [b.succ]) → ¬Arc w .cw (a.succ :: l2 ++ [b.succ])) :
+    (noKGon2Arc w.rlen sz1 sz2).eval (w.toPropAssn false) := by
+  simp [noKGon2Arc]; intro a b ab h1 h2
+  have ab : a < b := Nat.lt_of_le_of_lt (Nat.le_add_right ..) (Nat.add_assoc .. ▸ ab)
+  have ⟨l1, h11, h12⟩ := satisfies_arc2 ab h1
+  have ⟨l2, h21, h22⟩ := satisfies_arc2 ab h2
+  exact H _ _ _ _ h11 h21 h12 h22
+
+theorem hasConvex_of_σCCWPoints {w : CanonicalPoints} {l : List (Fin w.length)} (k3 : 3 ≤ k)
+    (H : σCCWPoints (l.map (w[·]))) (eq : l.length = k) : σHasConvexKGon k w.toFinset := by
+  refine (σHasConvexKGon_iff_HasConvexKGon w.gp).2
+    ⟨(l.map (w[·])).toFinset, Eq.trans ?_ eq, ?_, H.convex⟩
+  · show List.length _ = _; rw [dedup_eq_self.2, length_map]
+    apply H.gp.nodup; rwa [length_map, eq]
+  · simp [mem_points_iff]
+
+theorem satisfies_gonEncoding (w : CanonicalPoints) (k : Nat) :
+    ¬σHasConvexKGon k w.toFinset →
+    (gonEncoding k w.rlen).eval (w.toPropAssn false) := by
+  simp [gonEncoding, satisfies_baseEncoding, satisfies_signotopeClauses2,
+    satisfies_arcDefClausesUpTo, noGonClauses]
+  intro noholes k0
+  obtain ⟨k, rfl⟩ := Nat.exists_eq_add_of_le' k0
+  rw [show k+3-3 = k by rfl, show k+3-2 = k+1 by rfl]
+  refine ⟨?_, fun ⟨sz1, hsz⟩ => ?_⟩ <;> refine satisfies_noKGon2Arc fun a b l1 l2 h1 h2 h3 h4 => ?_
+  · have := Arc.join (l₁ := a.succ::l1) (l₂ := []) h3.cons_0 (.one (Nat.succ_pos _))
+    exact noholes <| hasConvex_of_σCCWPoints (Nat.le_add_left ..) this (by simp [h1])
+  · exact noholes <| hasConvex_of_σCCWPoints (Nat.le_add_left ..) (Arc.join h3 h4)
+      (by simp [h1, h2]; omega)
+
+end CanonicalPoints
