Lean/Geo/Gon/Encoding.lean
@@ -1,0 +1,47 @@
+import Mathlib.Data.Fin.Basic
+import Mathlib.Data.List.Range
+import Geo.SAT.ToLeanSAT.EncodeProof
+import Geo.KGon.Var
+import Geo.KGon.Encoding
+
+namespace Geo
+
+open LeanSAT Var
+
+def arc2 (o : Orientation) (sz : Nat) (a c : Fin n) : PropForm (Var n) :=
+  match sz with
+  | 0 => .true
+  | sz+1 =>
+    .atomic <| .flatCNF <|
+    .exists (Fin n) fun b =>
+    .andP (a.1+sz < b.1 ∧ b < c) fun _ =>
+    arc o sz a b c
+
+def noKGon2Arc (n sz1 sz2 : Nat) : PropForm (Var n) :=
+  .forAll (Fin n) fun a =>
+  .forAll (Fin n) fun b =>
+  .impP (a.1+sz1+sz2 < b.1) fun _ =>
+  .not <| .and (arc2 .ccw sz1 a b) (arc2 .cw sz2 a b)
+
+-- for k = 6:
+--
+-- 1            ..       ...       ....
+--  a     b   a    b   a     b   a      b
+--    ...       ..       .
+def noGonClauses (k n : Nat) : PropForm (Var n) :=
+  .impP (3 ≤ k) fun _ =>
+  .and (noKGon2Arc n (k-3) 0) <|
+  .forAll (Fin (k-3)) fun ⟨sz1, _⟩ =>
+  noKGon2Arc n sz1 (k-2-sz1)
+
+def gonEncoding (k n : Nat) : PropForm (Var n) :=
+  .all #[
+    baseEncoding n false, signotopeClauses2 n,
+    arcDefClausesUpTo n .ccw (k-4),
+    arcDefClausesUpTo n .cw (k-3),
+    noGonClauses k n]
+
+def gonCNF (k rlen : Nat) : ICnf := (Geo.gonEncoding k rlen |>.toICnf compare).2
+
+-- set_option profiler true in
+-- #eval let cnf := Geo.naiveCNF 10; (cnf.size, cnf.maxVar)
