Lean/Geo/Gon/TheMainTheorem.lean
@@ -1,0 +1,74 @@
+import Geo.Canonicalization.SymmetryBreaking
+import Geo.Gon.Assn
+import Geo.Gon.Encoding
+
+namespace Geo
+open Classical LeanSAT Model
+
+theorem gon_theorem (rlen_le : 2 ≤ rlen) (unsat : (Geo.gonCNF k rlen).isUnsat)
+    (pts : List Point) (gp : Point.ListInGenPos pts)
+    (h : pts.length ≥ rlen+1) : HasConvexKGon k pts.toFinset := by
+  refine HasConvexKGon_extension gp (fun pts gp h => ?_) h
+  by_contra h'
+  have noσgon : ¬σHasConvexKGon k pts.toFinset := mt (σHasConvexKGon_iff_HasConvexKGon gp).1 h'
+  have ⟨w, ⟨hw⟩⟩ := @symmetry_breaking pts (h ▸ Nat.succ_le_succ rlen_le) gp
+  have noσgon' : ¬σHasConvexKGon k w.toFinset :=
+    OrientationProperty_σHasConvexKGon.not (hw.toEquiv w.nodup) noσgon
+  have rlen9 : w.rlen = rlen := Nat.succ_inj.1 <| hw.length_eq.symm.trans h
+  apply unsat
+  with_reducible
+    have := (LeanSAT.PropForm.toICnf_sat _).2 ⟨w.toPropAssn _, w.satisfies_gonEncoding k noσgon'⟩
+    rw [rlen9] at this
+    rwa [gonCNF]
+
+/-- This asserts that the CNF produced by `lake exe encode gon 3 3 vars.out` is UNSAT -/
+axiom unsat_3gon_cnf : (Geo.gonCNF (k := 3) (rlen := 3-1)).isUnsat
+
+theorem gon_3_theorem : ∀ (pts : List Point),
+    Point.ListInGenPos pts → pts.length ≥ 3 → HasConvexKGon 3 pts.toFinset :=
+  gon_theorem (by decide) unsat_3gon_cnf
+
+/-- This asserts that the CNF produced by `lake exe encode gon 4 5 vars.out` is UNSAT -/
+axiom unsat_4gon_cnf : (Geo.gonCNF (k := 4) (rlen := 5-1)).isUnsat
+
+theorem gon_4_theorem : ∀ (pts : List Point),
+    Point.ListInGenPos pts → pts.length ≥ 5 → HasConvexKGon 4 pts.toFinset :=
+  gon_theorem (by decide) unsat_4gon_cnf
+
+/-- This asserts that the CNF produced by `lake exe encode gon 5 9 vars.out` is UNSAT -/
+axiom unsat_5gon_cnf : (Geo.gonCNF (k := 5) (rlen := 9-1)).isUnsat
+
+theorem gon_5_theorem : ∀ (pts : List Point),
+    Point.ListInGenPos pts → pts.length ≥ 9 → HasConvexKGon 5 pts.toFinset :=
+  gon_theorem (by decide) unsat_5gon_cnf
+
+/-- This asserts that the CNF produced by `lake exe encode gon 6 17 vars.out` is UNSAT -/
+axiom unsat_6gon_cnf : (Geo.gonCNF (k := 6) (rlen := 17-1)).isUnsat
+
+theorem gon_6_theorem : ∀ (pts : List Point),
+    Point.ListInGenPos pts → pts.length ≥ 17 → HasConvexKGon 6 pts.toFinset :=
+  gon_theorem (by decide) unsat_6gon_cnf
+
+/--
+info: 'Geo.gon_3_theorem' depends on axioms:
+[propext, Classical.choice, Quot.sound, mathlibSorry, Geo.unsat_3gon_cnf]
+-/
+#guard_msgs in #print axioms gon_3_theorem
+
+/--
+info: 'Geo.gon_4_theorem' depends on axioms:
+[propext, Classical.choice, Quot.sound, mathlibSorry, Geo.unsat_4gon_cnf]
+-/
+#guard_msgs in #print axioms gon_4_theorem
+
+/--
+info: 'Geo.gon_5_theorem' depends on axioms:
+[propext, Classical.choice, Quot.sound, mathlibSorry, Geo.unsat_5gon_cnf]
+-/
+#guard_msgs in #print axioms gon_5_theorem
+
+/--
+info: 'Geo.gon_6_theorem' depends on axioms:
+[propext, Classical.choice, Quot.sound, mathlibSorry, Geo.unsat_6gon_cnf]
+-/
+#guard_msgs in #print axioms gon_6_theorem
