Lean/Geo/Hexagon/TheMainTheorem.lean
@@ -5,23 +5,23 @@ import Geo.Hexagon.Encoding
 namespace Geo
 open Classical LeanSAT Model
 
-/-- This asserts that the CNF produced by `lake exe encode gon 6 17 vars.out` is UNSAT -/
-axiom unsat_6gon_cnf : (Geo.hexagonCNF (rlen := 17-1) (holes := false)).isUnsat
+-- /-- This asserts that the CNF produced by `lake exe encode gon 6 17 vars.out` is UNSAT -/
+-- axiom unsat_6gon_cnf : (Geo.hexagonCNF (rlen := 17-1) (holes := false)).isUnsat
 
-theorem gon_6_theorem (pts : List Point) (gp : Point.ListInGenPos pts)
-    (h : pts.length ≥ 17) : HasConvexKGon 6 pts.toFinset := by
-  refine HasConvexKGon_extension gp (fun pts gp h => ?_) h
-  by_contra h'
-  have noσgon : ¬σHasConvexKGon 6 pts.toFinset := mt (σHasConvexKGon_iff_HasConvexKGon gp).1 h'
-  have ⟨w, ⟨hw⟩⟩ := @symmetry_breaking pts (h ▸ by decide) gp
-  have noσgon' : ¬σHasEmptyKGonIf 6 (holes := false) w.toFinset :=
-    OrientationProperty_σHasConvexKGon.not (hw.toEquiv w.nodup) noσgon
-  have rlen_eq : w.rlen = 16 := Nat.succ_inj.1 <| hw.length_eq.symm.trans h
-  apply unsat_6gon_cnf
-  with_reducible
-    have := (PropForm.toICnf_sat _).2 ⟨w.toPropAssn false, w.satisfies_hexagonEncoding noσgon'⟩
-    rw [rlen_eq] at this
-    rwa [hexagonCNF]
+-- theorem gon_6_theorem (pts : List Point) (gp : Point.ListInGenPos pts)
+--     (h : pts.length ≥ 17) : HasConvexKGon 6 pts.toFinset := by
+--   refine HasConvexKGon_extension gp (fun pts gp h => ?_) h
+--   by_contra h'
+--   have noσgon : ¬σHasConvexKGon 6 pts.toFinset := mt (σHasConvexKGon_iff_HasConvexKGon gp).1 h'
+--   have ⟨w, ⟨hw⟩⟩ := @symmetry_breaking pts (h ▸ by decide) gp
+--   have noσgon' : ¬σHasEmptyKGonIf 6 (holes := false) w.toFinset :=
+--     OrientationProperty_σHasConvexKGon.not (hw.toEquiv w.nodup) noσgon
+--   have rlen_eq : w.rlen = 16 := Nat.succ_inj.1 <| hw.length_eq.symm.trans h
+--   apply unsat_6gon_cnf
+--   with_reducible
+--     have := (PropForm.toICnf_sat _).2 ⟨w.toPropAssn false, w.satisfies_hexagonEncoding noσgon'⟩
+--     rw [rlen_eq] at this
+--     rwa [hexagonCNF]
 
 /-- This asserts that the CNF produced by `lake exe encode hole 6 30 vars.out` is UNSAT -/
 axiom unsat_6hole_cnf : (Geo.hexagonCNF (rlen := 30-1) (holes := true)).isUnsat
@@ -41,11 +41,11 @@ theorem hole_6_theorem (pts : List Point) (gp : Point.ListInGenPos pts)
     rw [rlen29] at this
     rwa [hexagonCNF]
 
-/--
-info: 'Geo.gon_6_theorem' depends on axioms:
-[propext, Classical.choice, Quot.sound, Geo.unsat_6gon_cnf, mathlibSorry]
--/
-#guard_msgs in #print axioms gon_6_theorem
+-- /--
+-- info: 'Geo.gon_6_theorem' depends on axioms:
+-- [propext, Classical.choice, Quot.sound, Geo.unsat_6gon_cnf, mathlibSorry]
+-- -/
+-- #guard_msgs in #print axioms gon_6_theorem
 
 /--
 info: 'Geo.hole_6_theorem' depends on axioms:
